refactor: redesign `can_flow`

src/DY.Core.Label.Type.fst
@@ -1,27 +1,32 @@
 module DY.Core.Label.Type
 
-open DY.Core.Label.Lattice
+noeq
+type order (a:Type) = {
+  rel: a -> a -> prop;
+  refl: x:a -> Lemma (rel x x);
+  trans: x:a -> y:a -> z:a -> Lemma (requires rel x y /\ rel y z) (ensures rel x z);
+}
 
 type principal = string
 
-type pre_pre_label =
-  | P: principal -> pre_pre_label
-  | S: principal -> nat -> pre_pre_label
+type pre_label =
+  | P: principal -> pre_label
+  | S: principal -> nat -> pre_label
 
-val get_principal: pre_pre_label -> option principal
+val get_principal: pre_label -> option principal
 let get_principal l =
   match l with
   | P p -> Some p
   | S p _ -> Some p
 
-val get_session: pre_pre_label -> option nat
+val get_session: pre_label -> option nat
 let get_session l =
   match l with
   | P _ -> None
   | S _ s -> Some s
 
-val pre_pre_label_order: order pre_pre_label
-let pre_pre_label_order = {
+val pre_label_order: order pre_label
+let pre_label_order = {
   rel = (fun x y ->
     match y with
     | P p -> Some p == get_principal x
@@ -31,50 +36,9 @@ let pre_pre_label_order = {
   trans = (fun x y z -> ());
 }
 
-val corruption_pred_ok: #a:Type -> order a -> (a -> prop) -> prop
-let corruption_pred_ok #a ord pred =
-  forall x y. pred x /\ ord.rel x y ==> pred y
-
-type corruption_pred (#a:Type) (ord:order a) =
-  pred:(a -> prop){corruption_pred_ok ord pred}
-
-type pre_label (a:Type) =
-  | Secret: pre_label a
-  | State: a -> pre_label a
-  | Public: pre_label a
-
-val pre_label_order: #a:Type -> ord:order a -> corruption_pred ord  -> order (pre_label a)
-let pre_label_order ord is_corrupt = {
-  rel = (fun x y ->
-    match x, y with
-    | Secret, _ -> True
-    | _, Secret -> False
-    | State px, State py -> is_corrupt py \/ ord.rel px py
-    | State _, Public -> True
-    | Public, Public -> True
-    | Public, State py -> is_corrupt py
-  );
-  refl = (fun x ->
-    match x with
-    | State x0 -> ord.refl x0
-    | _ -> ()
-  );
-  trans = (fun x y z ->
-    match x, y, z with
-    | State x0, State y0, State z0 -> FStar.Classical.move_requires_3 ord.trans x0 y0 z0
-    | _, _, _ -> ()
-  );
-}
-
-type label = lattice (pre_label pre_pre_label)
-
-val label_order: corruption_pred pre_pre_label_order -> order label
-let label_order is_corrupt = {
-  rel = lattice_order (pre_label_order pre_pre_label_order is_corrupt);
-  refl = (fun x ->
-    lattice_order_refl (pre_label_order pre_pre_label_order is_corrupt) x
-  );
-  trans = (fun x y z ->
-    lattice_order_trans (pre_label_order pre_pre_label_order is_corrupt) x y z
-  );
-}
+type label =
+  | Secret: label
+  | State: pre_label -> label
+  | Meet: label -> label -> label
+  | Join: label -> label -> label
+  | Public: label
