src/DY.Core.fst
@@ -2,7 +2,6 @@ module DY.Core
 
 include DY.Core.Attacker.Knowledge
 include DY.Core.Label
-include DY.Core.Label.Lattice
 include DY.Core.Label.Type
 include DY.Core.Trace.Invariant
 include DY.Core.Trace.Manipulation
